update proofs and defs

ds_abs0/abs_relScript.sml
@@ -44,14 +44,27 @@ IS_ABS_STATE_REL (ds_abs0:ds_abs0_state) (ds_abs1:ds_abs1_state) =
 (ds_abs1.state = abs1_xfer_data) \/
 (ds_abs1.state = abs1_xfer_exchange))) /\
 ((ds_abs0.state = abs0_xfer_done) =
-((ds_abs1.state = abs1_xfer_update) /\
-(ds_abs1.state = abs1_xfer_ready) /\
+((ds_abs1.state = abs1_xfer_update) \/
+(ds_abs1.state = abs1_xfer_ready) \/
 (ds_abs1.state = abs1_xfer_fetch_data))))`
 
 (* abs_rel: ds_abs0_state -> ds_abs1_state -> bool *)
 val abs_rel_def = Define `
 abs_rel (ds_abs0:ds_abs0_state) (ds_abs1:ds_abs1_state) =
 ((ds_abs0.err = ds_abs1.err) /\
-(IS_ABS_STATE_REL ds_abs0 ds_abs1))`
+(IS_ABS_STATE_REL ds_abs0 ds_abs1) /\
+(ds_abs0.ds_abs0_tx.tx_data_buffer = ds_abs1.ds_abs1_tx.tx_data_buffer) /\
+(ds_abs0.ds_abs0_tx.tx_cur_length = ds_abs1.ds_abs1_tx.tx_cur_length) /\
+(ds_abs0.ds_abs0_rx.rx_data_buffer = ds_abs1.ds_abs1_rx.rx_data_buffer) /\
+(ds_abs0.ds_abs0_rx.rx_left_length = ds_abs1.ds_abs1_rx.rx_left_length) /\
+(ds_abs0.ds_abs0_xfer.xfer_dataIN_buffer = ds_abs1.ds_abs1_xfer.xfer_dataIN_buffer) /\
+(ds_abs0.ds_abs0_xfer.xfer_dataOUT_buffer = ds_abs1.ds_abs1_xfer.xfer_dataOUT_buffer) /\
+(ds_abs0.ds_abs0_xfer.xfer_cur_length = ds_abs1.ds_abs1_xfer.xfer_cur_length) /\
+(* some requirements for rx automaton *)
+(ds_abs0.state = abs0_rx_reading ==> ds_abs1.spi_abs1.RX_SHIFT_REG = ds_abs0.ds_abs0_rx.temp_RSR) /\
+(ds_abs0.state = abs0_rx_update ==> ds_abs1.spi_abs1.RX_SHIFT_REG = ds_abs0.ds_abs0_rx.temp_RSR) /\
+(ds_abs0.state = abs0_rx_next ==> ds_abs1.spi_abs1.RX_SHIFT_REG = ds_abs0.ds_abs0_rx.temp_RSR) /\
+(ds_abs0.state = abs0_rx_next ==> ds_abs1.ds_abs1_rx.temp_value = ds_abs0.ds_abs0_rx.temp_value) /\
+(ds_abs0.state = abs0_xfer_done ==> ds_abs1.spi_abs1.RX_SHIFT_REG = ds_abs0.ds_abs0_xfer.xfer_RSR))`
 
 val _ = export_theory();
