ds_abs0/ds_abs0_xferScript.sml
@@ -20,7 +20,7 @@ abs0_xfer_op (ds_abs0:ds_abs0_state) (data:word8 option) =
 if (data <> NONE) then
 (ds_abs0 with <| state := abs0_xfer_done;
 ds_abs0_xfer := ds_abs0.ds_abs0_xfer with
-<| xfer_dataIN_buffer := ds_abs0.ds_abs0_xfer.xfer_dataIN_buffer ++ [THE data];
+<| xfer_RSR := THE data;
 xfer_cur_length := ds_abs0.ds_abs0_xfer.xfer_cur_length + 1 |> |>,
 SOME (EL (ds_abs0.ds_abs0_xfer.xfer_cur_length) (ds_abs0.ds_abs0_xfer.xfer_dataOUT_buffer)))
 else (ds_abs0 with err := T, NONE)`
@@ -38,8 +38,10 @@ let (ds_abs0', dataOUT) = abs0_xfer_op ds_abs0 data in dataOUT`
 val abs0_xfer_tau_op_def = Define `
 abs0_xfer_tau_op (ds_abs0: ds_abs0_state) =
 ds_abs0 with
-state := if ds_abs0.ds_abs0_xfer.xfer_cur_length < 
+<| state := if ds_abs0.ds_abs0_xfer.xfer_cur_length < 
 (LENGTH ds_abs0.ds_abs0_xfer.xfer_dataOUT_buffer)
-then abs0_xfer_idle else abs0_ready`
+then abs0_xfer_idle else abs0_ready;
+ds_abs0_xfer := ds_abs0.ds_abs0_xfer with
+xfer_dataIN_buffer := ds_abs0.ds_abs0_xfer.xfer_dataIN_buffer ++ [ds_abs0.ds_abs0_xfer.xfer_RSR] |>`
 
 val _ = export_theory();
