ds_abs1/ds_abs1_relScript.sml
@@ -62,5 +62,37 @@ ds_abs1_tr ds_abs1 (RX data) (abs1_rx_receive_data_op ds_abs1 data)) /\
 ds_abs1_tr ds_abs1 (XFER dataIN (abs1_xfer_exchange_op_value ds_abs1 dataIN)) 
 (abs1_xfer_exchange_op_state ds_abs1 dataIN))`
 
+(* ds_abs1_tau_only_1_state: ds_abs1_state -> ds_abs1_state *)
+val ds_abs1_tau_only_1_state_def = Define `
+ds_abs1_tau_only_1_state (ds_abs1:ds_abs1_state) =
+((ds_abs1.state <> abs1_tx_trans) /\
+(ds_abs1.state <> abs1_tx_done_2) /\ 
+(ds_abs1.state <> abs1_rx_fetch_data) /\
+(ds_abs1.state <> abs1_rx_ready) /\
+(ds_abs1.state <> abs1_rx_next) /\
+(ds_abs1.state <> abs1_xfer_fetch_data))`
+
+(* An abstract transition system for ds_abs1 that removes some tau transition 
+val (ds_abs1_abs_tr_rules, ds_abs1_abs_tr_ind, ds_abs1_abs_tr_cases) = Hol_reln `
+(!(ds_abs1:ds_abs1_state). (ds_abs1_tr ds_abs1 tau ds_abs1') /\ 
+(ds_abs1_tr ds_abs1' lbl ds_abs1'') /\ (ds_abs1_tau_only_1_state ds_abs1) ==>
+ds_abs1_abs_tr ds_abs1 lbl ds_abs1'') /\
+(!(ds_abs1:ds_abs1_state). (ds_abs1_tr ds_abs1 tau ds_abs1') /\
+(ds_abs1.state = abs1_rx_ready \/ ds_abs1.state = abs1_xfer_fetch_data) ==>
+ds_abs1_abs_tr ds_abs1 tau ds_abs1') /\
+(!(ds_abs1:ds_abs1_state). (ds_abs1_tr ds_abs1 lbl ds_abs1') /\
+(ds_abs1.state = abs1_rx_fetch_data) ==>
+ds_abs1_abs_tr ds_abs1 lbl ds_abs1') /\
+(!(ds_abs1:ds_abs1_state). (ds_abs1_tr ds_abs1 tau ds_abs1') /\ (ds_abs1_tr ds_abs1 tau ds_abs1'') /\
+(ds_abs1' <> ds_abs1'') /\ (ds_abs1.state = abs1_tx_trans) /\
+(ds_abs1_abs_tr ds_abs1' lbl ds_abs1''') /\ (ds_abs1_abs_tr ds_abs1'' lbl ds_abs1''') ==>
+ds_abs1_abs_tr ds_abs1 lbl ds_abs1''') /\
+(!(ds_abs1:ds_abs1_state). (ds_abs1_tr ds_abs1 tau ds_abs1') /\ (ds_abs1_tr ds_abs1 tau ds_abs1'') /\
+(ds_abs1' <> ds_abs1'') /\ (ds_abs1.state = abs1_rx_next) /\
+(ds_abs1_tr ds_abs1' tau ds_abs1''') /\ (ds_abs1_tr ds_abs1'' tau ds_abs1''') /\ (ds_abs1_abs_tr ds_abs1''' lbl ds_abs1'''')  ==>
+ds_abs1_abs_tr ds_abs1 lbl ds_abs1'''') /\
+(!(ds_abs1:ds_abs1_state). (ds_abs1_tr ds_abs1 lbl ds_abs1') /\ (lbl <> tau) ==>
+ds_abs1_abs_tr ds_abs1 lbl ds_abs1')`
+ *)
 
 val _ = export_theory();
