abs0_abs1_thm/abs_rel_holds_abs1_tau_combScript.sml
@@ -1,0 +1,54 @@
+open HolKernel bossLib boolLib Parse;
+open SPI_stateTheory ds_abs1_stateTheory;
+open ds_abs0_relTheory abs_relTheory;
+open ds_abs1_relTheory ds_abs1_initTheory ds_abs1_txTheory ds_abs1_rxTheory ds_abs1_xferTheory;
+
+val _ = new_theory "abs_rel_holds_abs1_tau_comb";
+
+(* abs_rel holds for ds_abs1 tau_comb in the init automaton *)
+val abs_rel_holds_abs1_tau_comb_init = store_thm("abs_rel_holds_abs1_tau_comb_init",
+``!(ds_abs0:ds_abs0_state) (ds_abs1:ds_abs1_state).
+(abs_rel ds_abs0 ds_abs1) /\ (COMB_ABS1_INIT_ENABLE ds_abs1) ==>
+(abs_rel ds_abs0 (comb_abs1_init_operations ds_abs1))``,
+rw [COMB_ABS1_INIT_ENABLE_def, comb_abs1_init_operations_def, comb_abs1_init_start_op_def] >>
+fs [abs_rel_def, IS_ABS_STATE_REL_def]);
+
+(* abs_rel holds for ds_abs1 tau_comb in the tx automaton *)
+val abs_rel_holds_abs1_tau_comb_tx = store_thm("abs_rel_holds_abs1_tau_comb_tx",
+``!(ds_abs0:ds_abs0_state) (ds_abs1:ds_abs1_state).
+(abs_rel ds_abs0 ds_abs1) /\ (COMB_ABS1_TX_ENABLE ds_abs1) ==>
+(abs_rel ds_abs0 (comb_abs1_tx_operations ds_abs1))``,
+rw [COMB_ABS1_TX_ENABLE_def, comb_abs1_tx_operations_def] >>
+rw [comb_abs1_tx_trans_op_def, comb_abs1_tx_done_2_op_def, comb_abs1_tx_reset_op_def] >>
+fs [abs_rel_def, IS_ABS_STATE_REL_def] >> cheat);
+
+(* abs_rel holds for ds_abs1 tau_comb in the rx automaton *)
+val abs_rel_holds_abs1_tau_comb_rx = store_thm("abs_rel_holds_abs1_tau_comb_rx",
+``!(ds_abs0:ds_abs0_state) (ds_abs1:ds_abs1_state).
+(abs_rel ds_abs0 ds_abs1) /\ (COMB_ABS1_RX_ENABLE ds_abs1) ==>
+(abs_rel ds_abs0 (comb_abs1_rx_operations ds_abs1))``,
+rw [COMB_ABS1_RX_ENABLE_def, comb_abs1_rx_operations_def] >>
+rw [comb_abs1_rx_read_op_def, comb_abs1_rx_reset_op_def] >>
+fs [abs_rel_def, IS_ABS_STATE_REL_def]);
+
+(* abs_rel holds for ds_abs1 tau_comb in the xfer automaton *)
+val abs_rel_holds_abs1_tau_comb_xfer = store_thm("abs_rel_holds_abs1_tau_comb_xfer",
+``!(ds_abs0:ds_abs0_state) (ds_abs1:ds_abs1_state).
+(abs_rel ds_abs0 ds_abs1) /\ (COMB_ABS1_XFER_ENABLE ds_abs1) ==>
+(abs_rel ds_abs0 (comb_abs1_xfer_operations ds_abs1))``,
+rw [COMB_ABS1_XFER_ENABLE_def, comb_abs1_xfer_operations_def] >>
+rw [comb_abs1_xfer_prepare_op_def, comb_abs1_xfer_ready_op_def, 
+comb_abs1_xfer_reset_op_def] >>
+fs [abs_rel_def, IS_ABS_STATE_REL_def] >> cheat);
+
+(* abs_rel holds when ds_abs1 peforms tau_comb *)
+val abs_rel_holds_abs1_tau_comb = store_thm("abs_rel_holds_abs1_tau_comb",
+``!(ds_abs0:ds_abs0_state) (ds_abs1:ds_abs1_state) (ds_abs1':ds_abs1_state).
+(abs_rel ds_abs0 ds_abs1) /\ (ds_abs1_comb_tr ds_abs1 tau_comb ds_abs1') ==>
+(abs_rel ds_abs0 ds_abs1') \/
+(?ds_abs0'. ds_abs0_tr ds_abs0 tau ds_abs0' /\ abs_rel ds_abs0' ds_abs1')``,
+rw [ds_abs1_comb_tr_cases] >>
+rw [abs_rel_holds_abs1_tau_comb_init, abs_rel_holds_abs1_tau_comb_tx,
+abs_rel_holds_abs1_tau_comb_rx, abs_rel_holds_abs1_tau_comb_xfer]);
+
+val _ = export_theory();
