abs0_abs1_thm/abs_rel_holds_abs1_tau_drScript.sml
@@ -1,0 +1,66 @@
+open HolKernel bossLib boolLib Parse;
+open SPI_stateTheory ds_abs1_stateTheory;
+open ds_abs0_relTheory abs_relTheory ds_abs0_initTheory ds_abs0_txTheory ds_abs0_rxTheory ds_abs0_xferTheory ds_abs0_tauTheory;
+open ds_abs1_relTheory ds_abs1_initTheory ds_abs1_txTheory ds_abs1_rxTheory ds_abs1_xferTheory;
+
+val _ = new_theory "abs_rel_holds_abs1_tau_dr";
+
+(* abs_rel_holds for abs1 rx automaton tau_dr transition *)
+val abs_rel_holds_abs1_tau_dr_rx = store_thm("abs_rel_holds_abs1_tau_dr_rx",
+``!(ds_abs0:ds_abs0_state) (ds_abs1:ds_abs1_state).
+(abs_rel ds_abs0 ds_abs1) /\ (DRIVER_ABS1_RX_ENABLE ds_abs1) ==>
+?ds_abs0'. ds_abs0_tr ds_abs0 tau ds_abs0' /\ 
+abs_rel ds_abs0' (driver_abs1_rx_operations ds_abs1)``,
+rw [DRIVER_ABS1_RX_ENABLE_def, driver_abs1_rx_operations_def] >>
+`IS_ABS_STATE_REL ds_abs0 ds_abs1` by METIS_TAC [abs_rel_def] >|
+[(* abs1_rx_ready *)
+`ds_abs0.state = abs0_rx_update` by METIS_TAC [IS_ABS_STATE_REL_def] >>
+rw [driver_abs1_rx_ready_op_def] >|
+[`ds_abs0.ds_abs0_rx.rx_left_length > 0` by METIS_TAC [abs_rel_def] >>
+rw [ds_abs0_tr_cases, ABS0_TAU_LBL_ENABLE_def, abs0_tau_op_def, abs0_rx_update_op_def] >>
+fs [abs_rel_def, IS_ABS_STATE_REL_def],
+`~(ds_abs0.ds_abs0_rx.rx_left_length > 0)` by METIS_TAC [abs_rel_def] >>
+rw [ds_abs0_tr_cases, ABS0_TAU_LBL_ENABLE_def, abs0_tau_op_def, abs0_rx_update_op_def] >>
+fs [abs_rel_def, IS_ABS_STATE_REL_def]],
+(* abs1_rx_fetch_data *)
+`ds_abs0.state = abs0_rx_reading` by METIS_TAC [IS_ABS_STATE_REL_def] >>
+rw [driver_abs1_rx_fetch_data_op_def] >>
+rw [ds_abs0_tr_cases, ABS0_TAU_LBL_ENABLE_def, abs0_tau_op_def, abs0_rx_reading_op_def] >>
+fs [abs_rel_def, IS_ABS_STATE_REL_def],
+(* abs1_rx_next *)
+`ds_abs0.state = abs0_rx_next` by METIS_TAC [IS_ABS_STATE_REL_def] >>
+rw [driver_abs1_rx_next_op_def] >>
+rw [ds_abs0_tr_cases, ABS0_TAU_LBL_ENABLE_def, abs0_tau_op_def, abs0_rx_next_op_def] >>
+fs [abs_rel_def, IS_ABS_STATE_REL_def],
+(* abs1_rx_next_ready *)
+`ds_abs0.state = abs0_rx_next` by METIS_TAC [IS_ABS_STATE_REL_def] >>
+rw [driver_abs1_rx_next_ready_op_def] >>
+rw [ds_abs0_tr_cases, ABS0_TAU_LBL_ENABLE_def, abs0_tau_op_def, abs0_rx_next_op_def] >>
+fs [abs_rel_def, IS_ABS_STATE_REL_def]]);
+
+(* abs_rel_holds for abs1 xfer automaton tau_dr transition *)
+val abs_rel_holds_abs1_tau_dr_xfer = store_thm("abs_rel_holds_abs1_tau_dr_xfer",
+``!(ds_abs0:ds_abs0_state) (ds_abs1:ds_abs1_state).
+(abs_rel ds_abs0 ds_abs1) /\ (DRIVER_ABS1_XFER_ENABLE ds_abs1) ==>
+?ds_abs0'. ds_abs0_tr ds_abs0 tau ds_abs0' /\ 
+abs_rel ds_abs0' (driver_abs1_xfer_operations ds_abs1)``,
+rw [DRIVER_ABS1_XFER_ENABLE_def, driver_abs1_xfer_operations_def, driver_abs1_xfer_fetch_data_op_def] >>
+`IS_ABS_STATE_REL ds_abs0 ds_abs1` by METIS_TAC [abs_rel_def] >>
+`ds_abs0.state = abs0_xfer_done` by METIS_TAC [IS_ABS_STATE_REL_def] >|
+[`ds_abs0.ds_abs0_xfer.xfer_cur_length < LENGTH ds_abs0.ds_abs0_xfer.xfer_dataOUT_buffer` by METIS_TAC [abs_rel_def] >>
+rw [ds_abs0_tr_cases, ABS0_TAU_LBL_ENABLE_def, abs0_tau_op_def, abs0_xfer_tau_op_def] >>
+fs [abs_rel_def, IS_ABS_STATE_REL_def],
+`~ (ds_abs0.ds_abs0_xfer.xfer_cur_length < LENGTH ds_abs0.ds_abs0_xfer.xfer_dataOUT_buffer)` by METIS_TAC [abs_rel_def] >>
+rw [ds_abs0_tr_cases, ABS0_TAU_LBL_ENABLE_def, abs0_tau_op_def, abs0_xfer_tau_op_def] >>
+fs [abs_rel_def, IS_ABS_STATE_REL_def]]);
+
+(* abs_rel holds when ds_abs1 peforms tau_dr *)
+val abs_rel_holds_abs1_tau_dr = store_thm("abs_rel_holds_abs1_tau_dr",
+``!(ds_abs0:ds_abs0_state) (ds_abs1:ds_abs1_state) (ds_abs1':ds_abs1_state).
+(abs_rel ds_abs0 ds_abs1) /\ (ds_abs1_dr_tr ds_abs1 tau_dr ds_abs1') ==>
+(abs_rel ds_abs0 ds_abs1') \/
+(?ds_abs0'. ds_abs0_tr ds_abs0 tau ds_abs0' /\ abs_rel ds_abs0' ds_abs1')``,
+rw [ds_abs1_dr_tr_cases] >>
+rw [abs_rel_holds_abs1_tau_dr_rx, abs_rel_holds_abs1_tau_dr_xfer]);
+
+val _ = export_theory();
