abs0_abs1_thm/abs_rel_holds_call_lblScript.sml
@@ -1,0 +1,215 @@
+open HolKernel bossLib boolLib Parse;
+open SPI_stateTheory;
+open ds_abs0_relTheory abs_relTheory ds_abs0_initTheory ds_abs0_txTheory ds_abs0_rxTheory ds_abs0_xferTheory;
+open ds_abs1_relTheory ds_abs1_initTheory ds_abs1_txTheory ds_abs1_rxTheory ds_abs1_xferTheory;
+
+val _ = new_theory "abs_rel_holds_call_lbl";
+
+(* abs_rel holds for call_init label when ds_abs0 has call_init transition *)
+val abs0_abs_rel_call_init = store_thm("abs0_abs_rel_call_init",
+``!ds_abs0 ds_abs1 ds_abs0'.
+(abs_rel ds_abs0 ds_abs1) /\ (ABS0_CALL_INIT_ENABLE ds_abs0) ==>
+?ds_abs1'. (ds_abs1_abs_tr ds_abs1 call_init ds_abs1') /\ 
+(abs_rel (call_init_ds_abs0 ds_abs0) ds_abs1')``,
+rw [ABS0_CALL_INIT_ENABLE_def, call_init_ds_abs0_def] >>
+`IS_ABS_STATE_REL ds_abs0 ds_abs1` by METIS_TAC [abs_rel_def] >|
+[(* ds_abs0.state = abs0_init *)
+`ds_abs1.state = abs1_init_pre` by METIS_TAC [IS_ABS_STATE_REL_def] >>
+rw [ds_abs1_abs_tr_cases, ds_abs1_tr_cases] >>
+EXISTS_TAC ``call_init_ds_abs1 ds_abs1`` >>
+rw [call_init_ds_abs1_def] >>
+fs [abs_rel_def, IS_ABS_STATE_REL_def],
+(* ds_abs0.state = abs0_ready *)
+`ds_abs1.state = abs1_ready \/ ds_abs1.state = abs1_init_start \/
+ ds_abs1.state = abs1_tx_reset \/ ds_abs1.state = abs1_rx_reset \/
+ ds_abs1.state = abs1_xfer_reset` by METIS_TAC [IS_ABS_STATE_REL_def] >>
+rw [ds_abs1_abs_tr_cases, ds_abs1_tr_cases, ds_abs1_comb_tr_cases, 
+COMB_ABS1_INIT_ENABLE_def, COMB_ABS1_TX_ENABLE_def, COMB_ABS1_RX_ENABLE_def,
+COMB_ABS1_XFER_ENABLE_def, GSYM LEFT_EXISTS_AND_THM] >|
+[(* ds_abs1.state = abs1_ready *)
+EXISTS_TAC ``call_init_ds_abs1 ds_abs1`` >>
+rw [call_init_ds_abs1_def] >>
+fs [abs_rel_def, IS_ABS_STATE_REL_def],
+(* ds_abs1.state = abs1_init_start *)
+EXISTS_TAC ``comb_abs1_init_operations ds_abs1`` >>
+rw [comb_abs1_init_operations_def, comb_abs1_init_start_op_def, call_init_ds_abs1_def] >>
+fs [abs_rel_def, IS_ABS_STATE_REL_def],
+(* ds_abs1.state = abs1_tx_reset *)
+EXISTS_TAC ``comb_abs1_tx_operations ds_abs1`` >>
+rw [comb_abs1_tx_operations_def, comb_abs1_tx_reset_op_def, call_init_ds_abs1_def] >>
+fs [abs_rel_def, IS_ABS_STATE_REL_def],
+(* ds_abs1.state = abs1_rx_reset *)
+EXISTS_TAC ``comb_abs1_rx_operations ds_abs1`` >>
+rw [comb_abs1_rx_operations_def, comb_abs1_rx_reset_op_def, call_init_ds_abs1_def] >>
+fs [abs_rel_def, IS_ABS_STATE_REL_def],
+(* ds_abs1.state = abs1_xfer_reset *)
+EXISTS_TAC ``comb_abs1_xfer_operations ds_abs1`` >>
+rw [comb_abs1_xfer_operations_def, comb_abs1_xfer_reset_op_def, call_init_ds_abs1_def] >>
+fs [abs_rel_def, IS_ABS_STATE_REL_def]]]);
+
+(* abs_rel holds for call_tx label when ds_abs0 has call_tx transition *)
+val abs0_abs_rel_call_tx = store_thm("abs0_abs_rel_call_tx",
+``!ds_abs0 ds_abs1 buffer.
+(abs_rel ds_abs0 ds_abs1) /\ (ds_abs0.state = abs0_ready) /\ (buffer <> []) ==>
+?ds_abs1'. (ds_abs1_abs_tr ds_abs1 (call_tx buffer) ds_abs1') /\ 
+(abs_rel (call_tx_ds_abs0 ds_abs0 buffer) ds_abs1')``,
+rw [call_tx_ds_abs0_def] >>
+`IS_ABS_STATE_REL ds_abs0 ds_abs1` by METIS_TAC [abs_rel_def] >>
+`ds_abs1.state = abs1_ready \/ ds_abs1.state = abs1_init_start \/
+ ds_abs1.state = abs1_tx_reset \/ ds_abs1.state = abs1_rx_reset \/
+ ds_abs1.state = abs1_xfer_reset` by METIS_TAC [IS_ABS_STATE_REL_def] >>
+rw [ds_abs1_abs_tr_cases, ds_abs1_tr_cases, ds_abs1_comb_tr_cases, 
+COMB_ABS1_INIT_ENABLE_def, COMB_ABS1_TX_ENABLE_def, COMB_ABS1_RX_ENABLE_def,
+COMB_ABS1_XFER_ENABLE_def, GSYM LEFT_EXISTS_AND_THM] >|
+[(* ds_abs1.state = abs1_ready *)
+EXISTS_TAC ``call_tx_ds_abs1 ds_abs1 buffer`` >>
+rw [call_tx_ds_abs1_def] >>
+fs [abs_rel_def, IS_ABS_STATE_REL_def],
+(* ds_abs1.state = abs1_init_start *)
+EXISTS_TAC ``comb_abs1_init_operations ds_abs1`` >>
+rw [comb_abs1_init_operations_def, comb_abs1_init_start_op_def, call_tx_ds_abs1_def] >>
+fs [abs_rel_def, IS_ABS_STATE_REL_def],
+(* ds_abs1.state = abs1_tx_reset *)
+EXISTS_TAC ``comb_abs1_tx_operations ds_abs1`` >>
+rw [comb_abs1_tx_operations_def, comb_abs1_tx_reset_op_def, call_tx_ds_abs1_def] >>
+fs [abs_rel_def, IS_ABS_STATE_REL_def],
+(* ds_abs1.state = abs1_rx_reset *)
+EXISTS_TAC ``comb_abs1_rx_operations ds_abs1`` >>
+rw [comb_abs1_rx_operations_def, comb_abs1_rx_reset_op_def, call_tx_ds_abs1_def] >>
+fs [abs_rel_def, IS_ABS_STATE_REL_def],
+(* ds_abs1.state = abs1_xfer_reset *)
+EXISTS_TAC ``comb_abs1_xfer_operations ds_abs1`` >>
+rw [comb_abs1_xfer_operations_def, comb_abs1_xfer_reset_op_def, call_tx_ds_abs1_def] >>
+fs [abs_rel_def, IS_ABS_STATE_REL_def]]);
+
+(* abs_rel holds for call_rx label when ds_abs0 has call_rx transition *)
+val abs0_abs_rel_call_rx = store_thm("abs0_abs_rel_call_rx",
+``!ds_abs0 ds_abs1 length.
+(abs_rel ds_abs0 ds_abs1) /\ (ds_abs0.state = abs0_ready) /\ (length > 0) ==>
+?ds_abs1'. (ds_abs1_abs_tr ds_abs1 (call_rx length) ds_abs1') /\
+(abs_rel (call_rx_ds_abs0 ds_abs0 length) ds_abs1')``,
+rw [call_rx_ds_abs0_def] >>
+`IS_ABS_STATE_REL ds_abs0 ds_abs1` by METIS_TAC [abs_rel_def] >>
+`ds_abs1.state = abs1_ready \/ ds_abs1.state = abs1_init_start \/
+ ds_abs1.state = abs1_tx_reset \/ ds_abs1.state = abs1_rx_reset \/
+ ds_abs1.state = abs1_xfer_reset` by METIS_TAC [IS_ABS_STATE_REL_def] >>
+rw [ds_abs1_abs_tr_cases, ds_abs1_tr_cases, ds_abs1_comb_tr_cases, 
+COMB_ABS1_INIT_ENABLE_def, COMB_ABS1_TX_ENABLE_def, COMB_ABS1_RX_ENABLE_def,
+COMB_ABS1_XFER_ENABLE_def, GSYM LEFT_EXISTS_AND_THM] >|
+[(* abs1_ready *)
+EXISTS_TAC ``call_rx_ds_abs1 ds_abs1 length`` >>
+rw [call_rx_ds_abs1_def] >>
+fs [abs_rel_def, IS_ABS_STATE_REL_def],
+(* abs1_init_start *)
+EXISTS_TAC ``comb_abs1_init_operations ds_abs1`` >>
+rw [comb_abs1_init_operations_def, comb_abs1_init_start_op_def, call_rx_ds_abs1_def] >>
+fs [abs_rel_def, IS_ABS_STATE_REL_def],
+(* abs1_tx_reset *)
+EXISTS_TAC ``comb_abs1_tx_operations ds_abs1`` >>
+rw [comb_abs1_tx_operations_def, comb_abs1_tx_reset_op_def, call_rx_ds_abs1_def] >>
+fs [abs_rel_def, IS_ABS_STATE_REL_def],
+(* abs1_rx_reset *)
+EXISTS_TAC ``comb_abs1_rx_operations ds_abs1`` >>
+rw [comb_abs1_rx_operations_def, comb_abs1_rx_reset_op_def, call_rx_ds_abs1_def] >>
+fs [abs_rel_def, IS_ABS_STATE_REL_def],
+(* abs1_xfer_reset *)
+EXISTS_TAC ``comb_abs1_xfer_operations ds_abs1`` >>
+rw [comb_abs1_xfer_operations_def, comb_abs1_xfer_reset_op_def, call_rx_ds_abs1_def] >>
+fs [abs_rel_def, IS_ABS_STATE_REL_def]]);
+
+(* abs_rel holds for call_xfer label when ds_abs0 has call_xfer transition *)
+val abs0_abs_rel_call_xfer = store_thm("abs0_abs_rel_call_xfer",
+``!ds_abs0 ds_abs1 buffer.
+(abs_rel ds_abs0 ds_abs1) /\ (ds_abs0.state = abs0_ready) /\ (buffer <> []) ==>
+?ds_abs1'. (ds_abs1_abs_tr ds_abs1 (call_xfer buffer) ds_abs1') /\ 
+(abs_rel (call_xfer_ds_abs0 ds_abs0 buffer) ds_abs1')``,
+rw [call_xfer_ds_abs0_def] >>
+`IS_ABS_STATE_REL ds_abs0 ds_abs1` by METIS_TAC [abs_rel_def] >>
+`ds_abs1.state = abs1_ready \/ ds_abs1.state = abs1_init_start \/
+ ds_abs1.state = abs1_tx_reset \/ ds_abs1.state = abs1_rx_reset \/
+ ds_abs1.state = abs1_xfer_reset` by METIS_TAC [IS_ABS_STATE_REL_def] >>
+rw [ds_abs1_abs_tr_cases, ds_abs1_tr_cases, ds_abs1_comb_tr_cases, 
+COMB_ABS1_INIT_ENABLE_def, COMB_ABS1_TX_ENABLE_def, COMB_ABS1_RX_ENABLE_def,
+COMB_ABS1_XFER_ENABLE_def, GSYM LEFT_EXISTS_AND_THM] >|
+[(* abs1_ready *)
+EXISTS_TAC ``call_xfer_ds_abs1 ds_abs1 buffer`` >>
+rw [call_xfer_ds_abs1_def] >>
+fs [abs_rel_def, IS_ABS_STATE_REL_def],
+(* abs1_init_start *)
+EXISTS_TAC ``comb_abs1_init_operations ds_abs1`` >>
+rw [comb_abs1_init_operations_def, comb_abs1_init_start_op_def, call_xfer_ds_abs1_def] >>
+fs [abs_rel_def, IS_ABS_STATE_REL_def],
+(* abs1_tx_reset *)
+EXISTS_TAC ``comb_abs1_tx_operations ds_abs1`` >>
+rw [comb_abs1_tx_operations_def, comb_abs1_tx_reset_op_def, call_xfer_ds_abs1_def] >>
+fs [abs_rel_def, IS_ABS_STATE_REL_def],
+(* abs1_rx_reset *)
+EXISTS_TAC ``comb_abs1_rx_operations ds_abs1`` >>
+rw [comb_abs1_rx_operations_def, comb_abs1_rx_reset_op_def, call_xfer_ds_abs1_def] >>
+fs [abs_rel_def, IS_ABS_STATE_REL_def],
+(* abs1_xfer_reset *)
+EXISTS_TAC ``comb_abs1_xfer_operations ds_abs1`` >>
+rw [comb_abs1_xfer_operations_def, comb_abs1_xfer_reset_op_def, call_xfer_ds_abs1_def] >>
+fs [abs_rel_def, IS_ABS_STATE_REL_def]]);
+
+(* abs_rel holds for call_init label when ds_abs1 state is abs1_init_pre *)
+val abs1_init_pre_abs_rel_call_init = store_thm("abs1_init_pre_abs_rel_call_init",
+``!ds_abs0 ds_abs1.
+(abs_rel ds_abs0 ds_abs1) /\ (ds_abs1.state = abs1_init_pre) ==>
+?ds_abs0'. (ds_abs0_tr ds_abs0 call_init ds_abs0') /\ 
+(abs_rel ds_abs0' (call_init_ds_abs1 ds_abs1))``,
+rw [call_init_ds_abs1_def] >>
+`IS_ABS_STATE_REL ds_abs0 ds_abs1` by METIS_TAC [abs_rel_def] >>
+`ds_abs0.state = abs0_init` by METIS_TAC [IS_ABS_STATE_REL_def] >>
+rw [ds_abs0_tr_cases, ABS0_CALL_INIT_ENABLE_def, call_init_ds_abs0_def] >>
+fs [abs_rel_def, IS_ABS_STATE_REL_def]);
+
+(* abs_rel holds for call_init label when ds_abs1 state is abs1_ready *)
+val abs1_ready_abs_rel_call_init = store_thm("abs1_ready_abs_rel_call_init",
+``!ds_abs0 ds_abs1.
+(abs_rel ds_abs0 ds_abs1) /\ (ds_abs1.state = abs1_ready) ==>
+?ds_abs0'. (ds_abs0_tr ds_abs0 call_init ds_abs0') /\ 
+(abs_rel ds_abs0' (call_init_ds_abs1 ds_abs1))``,
+rw [call_init_ds_abs1_def] >>
+`IS_ABS_STATE_REL ds_abs0 ds_abs1` by METIS_TAC [abs_rel_def] >>
+`ds_abs0.state = abs0_ready` by METIS_TAC [IS_ABS_STATE_REL_def] >>
+rw [ds_abs0_tr_cases, ABS0_CALL_INIT_ENABLE_def, call_init_ds_abs0_def] >>
+fs [abs_rel_def, IS_ABS_STATE_REL_def]);
+
+(* abs_rel holds for call_tx label when ds_abs1 has call_tx transition *)
+val abs1_abs_rel_call_tx = store_thm("abs1_abs_rel_call_tx",
+``!ds_abs0 ds_abs1 buffer.
+(abs_rel ds_abs0 ds_abs1) /\ (ds_abs1.state = abs1_ready) /\ (buffer <> []) ==>
+?ds_abs0'. (ds_abs0_tr ds_abs0 (call_tx buffer) ds_abs0') /\
+(abs_rel ds_abs0' (call_tx_ds_abs1 ds_abs1 buffer))``,
+rw [call_tx_ds_abs1_def] >>
+`IS_ABS_STATE_REL ds_abs0 ds_abs1` by METIS_TAC [abs_rel_def] >>
+`ds_abs0.state = abs0_ready` by METIS_TAC [IS_ABS_STATE_REL_def] >>
+rw [ds_abs0_tr_cases, call_tx_ds_abs0_def] >>
+fs [abs_rel_def, IS_ABS_STATE_REL_def]);
+
+(* abs_rel holds for call_rx label when ds_abs1 has call_rx transition *)
+val abs1_abs_rel_call_rx = store_thm("abs1_abs_rel_call_rx",
+``!ds_abs0 ds_abs1 length.
+(abs_rel ds_abs0 ds_abs1) /\ (ds_abs1.state = abs1_ready) /\ (length > 0) ==>
+?ds_abs0'. (ds_abs0_tr ds_abs0 (call_rx length) ds_abs0') /\
+(abs_rel ds_abs0' (call_rx_ds_abs1 ds_abs1 length))``,
+rw [call_rx_ds_abs1_def] >>
+`IS_ABS_STATE_REL ds_abs0 ds_abs1` by METIS_TAC [abs_rel_def] >>
+`ds_abs0.state = abs0_ready` by METIS_TAC [IS_ABS_STATE_REL_def] >>
+rw [ds_abs0_tr_cases, call_rx_ds_abs0_def] >>
+fs [abs_rel_def, IS_ABS_STATE_REL_def]);
+
+(* abs_rel holds for call_xfer label when ds_abs1 has call_xfer transition *)
+val abs1_abs_rel_call_xfer = store_thm("abs1_abs_rel_call_xfer",
+``!ds_abs0 ds_abs1 buffer.
+(abs_rel ds_abs0 ds_abs1) /\ (ds_abs1.state = abs1_ready) /\ (buffer <> []) ==>
+?ds_abs0'. (ds_abs0_tr ds_abs0 (call_xfer buffer) ds_abs0') /\
+(abs_rel ds_abs0' (call_xfer_ds_abs1 ds_abs1 buffer))``,
+rw [call_xfer_ds_abs1_def] >>
+`IS_ABS_STATE_REL ds_abs0 ds_abs1` by METIS_TAC [abs_rel_def] >>
+`ds_abs0.state = abs0_ready` by METIS_TAC [IS_ABS_STATE_REL_def] >>
+rw [ds_abs0_tr_cases, call_xfer_ds_abs0_def] >>
+fs [abs_rel_def, IS_ABS_STATE_REL_def]);
+
+val _ = export_theory();
