abs0_abs1_thm/abs_weak_bisimulationScript.sml
@@ -1,0 +1,31 @@
+open HolKernel bossLib boolLib Parse;
+open SPI_stateTheory;
+open ds_abs0_relTheory abs_relTheory;
+open ds_abs1_relTheory;
+open abs_rel_holds_call_lblTheory;
+
+val _ = new_theory "abs_weak_bisimulation";
+
+(* weak bisimulation between ds_abs0 and ds_abs1 *)
+(* have to rewrite *)
+val abs0_weak_bisimulation = store_thm("abs0_weak_bisimulation",
+``!ds_abs0 ds_abs1 lbl ds_abs0'.
+(abs_rel ds_abs0 ds_abs1) /\ (ds_abs0_tr ds_abs0 lbl ds_abs0') ==>
+?ds_abs1'. (ds_abs1_abs_tr ds_abs1 lbl ds_abs1') /\ (abs_rel ds_abs0' ds_abs1')``,
+rw [ds_abs0_tr_cases] >>
+rw [abs0_abs_rel_call_init, abs0_abs_rel_call_tx, abs0_abs_rel_call_rx,
+abs0_abs_rel_call_xfer] >>
+cheat);
+
+
+val abs1_weak_bisimulation = store_thm("abs1_weak_bisimulation",
+``!ds_abs0 ds_abs1 lbl ds_abs1'.
+(abs_rel ds_abs0 ds_abs1) /\ (ds_abs1_tr ds_abs1 lbl ds_abs1') ==>
+(abs_rel ds_abs0 ds_abs1') \/
+(?ds_abs0'. (ds_abs0_tr ds_abs0 lbl ds_abs0') /\ (abs_rel ds_abs0' ds_abs1'))``,
+rw [ds_abs1_tr_cases] >>
+rw [abs1_init_pre_abs_rel_call_init, abs1_ready_abs_rel_call_init, 
+abs1_abs_rel_call_tx, abs1_abs_rel_call_rx, abs1_abs_rel_call_xfer] >>
+cheat);
+
+val _ = export_theory();
