abs0_abs1_thm/ds_abs1_tauScript.sml
@@ -1,0 +1,74 @@
+open HolKernel bossLib boolLib Parse;
+open SPI_stateTheory;
+open ds_abs1_relTheory ds_abs1_initTheory ds_abs1_txTheory ds_abs1_rxTheory ds_abs1_xferTheory;
+
+val _ = new_theory "ds_abs1_tau";
+
+(* Theorem: for most states with tau transitions,
+   tau is the only possible transition label *)
+val ds_abs1_only_tau = store_thm("ds_abs1_only_tau",
+``!ds_abs1 ds_abs1' ds_abs1'' lbl.
+(ds_abs1.state <> abs1_tx_done_2) /\ (ds_abs1.state <> abs1_rx_fetch_data) ==>
+(ds_abs1_tr ds_abs1 tau ds_abs1') ==>
+(ds_abs1_tr ds_abs1 lbl ds_abs1'') ==>
+lbl = tau ``,
+rw [ds_abs1_tr_cases] >>
+fs [ABS1_TX_LBL_ENABLE_def, ABS1_RX_LBL_ENABLE_def] >>
+fs [ds_abs1_spi_tr_cases, SPI_ABS1_TX_ENABLE_def, SPI_ABS1_RX_ENABLE_def, 
+SPI_ABS1_XFER_ENABLE_def, ds_abs1_dr_tr_cases,  DRIVER_ABS1_RX_ENABLE_def, 
+DRIVER_ABS1_XFER_ENABLE_def, ds_abs1_comb_tr_cases, COMB_ABS1_INIT_ENABLE_def, 
+COMB_ABS1_TX_ENABLE_def, COMB_ABS1_RX_ENABLE_def, COMB_ABS1_XFER_ENABLE_def]);
+
+(* For some states that have tau transitions, there is only 1 possible next state*)
+val ds_abs1_only_1_state_if_tau = store_thm("ds_abs1_only_1_state_if_tau",
+``!ds_abs1 ds_abs1' ds_abs1''.
+(ds_abs1_tau_only_1_state ds_abs1) ==>
+(ds_abs1_tr ds_abs1 tau ds_abs1') ==>
+(ds_abs1_tr ds_abs1 tau ds_abs1'') ==>
+ds_abs1' = ds_abs1''``,
+rw [ds_abs1_tr_cases, ds_abs1_tau_only_1_state_def] >>
+Cases_on `ds_abs1.state` >>
+rw [] >>
+fs [ds_abs1_spi_tr_cases, SPI_ABS1_TX_ENABLE_def, SPI_ABS1_RX_ENABLE_def, 
+SPI_ABS1_XFER_ENABLE_def, ds_abs1_dr_tr_cases,  DRIVER_ABS1_RX_ENABLE_def, 
+DRIVER_ABS1_XFER_ENABLE_def, ds_abs1_comb_tr_cases, COMB_ABS1_INIT_ENABLE_def, 
+COMB_ABS1_TX_ENABLE_def, COMB_ABS1_RX_ENABLE_def, COMB_ABS1_XFER_ENABLE_def] >>
+rw []);
+
+(* Theorem: for some states, tau is the only label and there is only 1 possible next state *)
+val ds_abs1_only_1_state_and_tau = store_thm("ds_abs1_only_1_state_and_tau",
+``!ds_abs1 ds_abs1' ds_abs1'' lbl.
+(ds_abs1_tau_only_1_state ds_abs1) ==>
+(ds_abs1_tr ds_abs1 tau ds_abs1') ==>
+(ds_abs1_tr ds_abs1 lbl ds_abs1'') ==>
+(lbl = tau) /\ (ds_abs1' = ds_abs1'')``,
+rw [] >|
+[METIS_TAC [ds_abs1_only_tau, ds_abs1_tau_only_1_state_def],
+`lbl = tau` by METIS_TAC [ds_abs1_only_tau, ds_abs1_tau_only_1_state_def] >>
+fs [] >>
+METIS_TAC [ds_abs1_only_1_state_if_tau]]);
+
+(*
+only_1_tau tr s1 s2 equal
+ tr s1 tau s2 and
+ !lbl2 s3 . tr s1 lbl2 S3 ==>
+  s1 equal S3
+   and lbl2 equal tau  
+ !lbl4 s4 . tr s4 lbl4 s2 implies
+  lbl4 equal tau 
+
+simplify tr1 tr2 s1 s2 define as
+
+
+
+Hol_reln simplify tr s1 s2 
+only_1_tau tr s1 s2 and exists lbl s3. tr s2 lbl s3
+  then simplify tr s1 lbl s3
+only_1_tau tr s1 s2 and exists s3. tr s3 tau s2
+  then simplify tr s3 lbl s1
+!s3 s4. s1 neq s3 and s1 neq s4 and tr s3 lbl s4 then
+ simplify tr s3 lbl s4
+*)
+
+
+val _ = export_theory();
